providers/evercrypt/EverCrypt.Vale.fsti
@@ -7,6 +7,11 @@ open EverCrypt.Helpers
 /// This module directly exposes "raw" functions, using attributes to make sure
 /// KreMLin generates the right "extern stdcall" declarations. There is no C code to implement this module, the implementations are provided at link-time.
 
+// Can't use the real ASM names because they are capitalized...
+// name forwarding is in evercrypt_vale_stubs.c with stdcall calls
+val aes128_key_expansion: key:uint8_p -> w:uint8_p -> sbox:uint8_p -> Stack_ unit
+val aes128_encrypt_one_block: cipher:uint8_p -> plain: uint8_p -> w:uint8_p -> sbox: uint8_p -> Stack_ unit
+
 noeq
 type gcm_args = {
   plain: uint8_p;
